Makefile
@@ -6,62 +6,44 @@ COQBIN=
 COQC=$(COQBIN)coqc
 COQDEP=$(COQBIN)coqdep
 
-Reentry_PREFIX = AST ASTLc Hoare HoareLc
+DIRS = WithCall WithoutCall
 
-WithoutCall_FILES = \
-	$(foreach prefix, $(Reentry_PREFIX), $(prefix)_woc.v)
+INCLUDE_DEMO = $(foreach d, $(DIRS), -R $(CURRENT_DIR)/$(d) Reentry.$(d))
+COQ_FLAG = $(INCLUDE_DEMO)
+DEP_DEMO = -R $(CURRENT_DIR) Reentry
+DEP_FLAG = $(DEP_DEMO)
 
-WithCall_FILES = \
-	$(foreach prefix, $(Reentry_PREFIX), $(prefix)_wc.v)
+Derivation_FILES = DenotationalSemantics.v FineGrainedSemantics.v DerivationTheorem.v
 
-Relation_PREFIX = \
-	DSRelation HRelation
+WithoutCall_FILES = $(Derivation_FILES)
 
-Unified_FILES = \
-	AST.v Label.v ASTLc.v Hoare.v HoareLc.v \
-	$(foreach prefix, $(Relation_PREFIX), $(prefix)_woc.v $(prefix)_wc.v)
-
-HoareFunc_FILES = \
-	HoareFunc.v
-
-FuncPredicate_FILES = \
-	AST_wc.v Hoare_wc.v $(HoareFunc_FILES)
+WithCall_FILES = $(Derivation_FILES) CoarseGrainedLogic.v
 
 FILES = \
-	$(WithoutCall_FILES) $(WithCall_FILES) $(HoareFunc_FILES) $(Unified_FILES)
+	$(WithoutCall_FILES:%.v=WithoutCall/%.v) \
+	$(WithCall_FILES:%.v=WithCall/%.v)
 
 $(FILES:%.v=%.vo): %.vo: %.v
 	@echo COQC $*.v
-	@$(COQC) $(CURRENT_DIR)/$*.v
-#	@$(COQC) $(COQ_FLAG) $(CURRENT_DIR)/$*.v
+	@$(COQC) $(COQ_FLAG) $(CURRENT_DIR)/$*.v
 
 WithoutCall: \
-	.depend $(WithoutCall_FILES:%.v=%.vo)
+	.depend clean $(WithoutCall_FILES:%.v=WithoutCall/%.vo)
 
 WithCall: \
-	.depend $(WithCall_FILES:%.v=%.vo)
-
-Unified: \
-	.depend $(Unified_FILES:%.v=%.vo)
-
-FuncPred: \
-	.depend $(FuncPredicate_FILES:%.v=%.vo)
+	.depend clean $(WithCall_FILES:%.v=WithCall/%.vo)
 
 all: $(FILES:%.v=%.vo)
 
 depend:
-	$(COQDEP) $(FILES) > .depend
-#	$(COQDEP) $(DEP_FLAG) $(FILES) > .depend
+	$(COQDEP) $(DEP_FLAG) $(FILES) > .depend
 
 .depend:
-	@$(COQDEP) $(FILES) > .depend
-#	@$(COQDEP) $(DEP_FLAG) $(FILES) > .depend
+	@$(COQDEP) $(DEP_FLAG) $(FILES) > .depend
 
 clean:
-	@rm *.vo *.glob .*.aux
+	@rm -f */.*.aux */*.vo */*.glob
 
-.DEFAULT_GOAL := WithoutCall
+.DEFAULT_GOAL := WithCall
 
-include .depend
-	
-	
+include .depend	
